% !TEX root = ../vr_st.tex

\subsection{Sums and products}\label{ss:sums_products}

\subsubsection{}

The \defn{wedge sum} of two pointed $\R$-spaces $X$ and $Y$ is defined by
\[
(X \vee Y)_r = X_r \vee Y_r \quad\text{and}\quad (X \vee Y)_{s,t} = (X_{s,t} \vee Y_{s,t})
\]
where \(r,s,t \in \R\) and \(s \leq t\).

Since for any \(r \in \R\), the natural inclusions $X_r \to X_r \vee Y_r \leftarrow Y_r$ induce an isomorphism $\rH^*(X_r \vee Y_r) \to \rH^*(X_r) \oplus \rH^*(Y_r)$ (\cite[Cor.~2.25.]{hatcher2000}), we have the following.

\medskip\lemma
Let $X$ and $Y$ be pointed cellular $\R$-spaces.
For any linear cohomology operation $\theta$:
\begin{align*}
	\img_\theta(X \vee Y) &\cong \img_\theta(X) \oplus \img_\theta(Y), \\
	\ker_\theta(X \vee Y) &\cong \ker_\theta(X) \oplus \ker_\theta(Y).
\end{align*}

%\begin{proof}
%
%	The claim follows from the naturality of \(\theta\).\anibal{note to self: Say more?}
%%	By the naturality of $\theta$ we have that $\theta_{X \vee Y} \circ (\iota^*_X \oplus \iota^*_Y) = (\iota^*_X \circ \theta_X) \oplus (\iota^*_Y \circ \theta_Y)$.
%%	So, $\img\theta_{X \vee Y} \cong \img\theta_X \oplus \img\theta_Y$ and $\ker\theta_{X \vee Y} \cong \ker\theta_X \oplus \ker\theta_Y$.
%\end{proof}

\subsubsection{}\label{ss:wedge sum}

The \defn{gluing metric} on the wedge sum of pointed metric spaces ${(\cX_i, x_i)}_{i = 0}^k$ is defined as follows: For $x \in \cX_i$ and $x' \in \cX_j$, let
\[
d(x, x') =
\begin{cases}
	d_{\cX_i}(x, x_i) + d_{\cX_j}(x', x_j) & i \neq j, \\
	\hfil d_{\cX_i}(x, x') & i = j.
\end{cases}
\]
%if $i \neq j$, and
%\[
%d(x, x') = d_{\cX_i}(x, x')
%\]
%if $i =j$,

\medskip\theorem
Let $\cX$ and $\cY$ be pointed metric spaces.
For any linear cohomology operation $\theta$:
\begin{align*}
	\img_\theta^\VR(\cX \vee \cY) &\cong \img_\theta^\VR(\cX) \oplus \img_\theta^\VR(\cY), \\
	\ker_\theta^\VR(\cX \vee \cY) &\cong \ker_\theta^\VR(\cX) \oplus \ker_\theta^\VR(\cY),
\end{align*}
where \(\cX \vee \cY\) is equipped with the gluing metric.

\begin{proof}
	This follows from the previous lemma and the fact, proven in \cite[Prop.~1]{adamaszek2020homotopy}, that the natural inclusion
	\[
	\VR_r(\cX) \vee \VR_r(\cY) \to \VR_r(\cX \vee \cY)
	\]
	is a homotopy equivalence for each $r \in \R$.
\end{proof}

\subsubsection{}

Similarly, for any two $\R$-spaces $X$ and $Y$, the $\R$-space $X \times Y$, their \defn{product}, is defined by
\[
(X \times Y)_r = X_r \times Y_r \quad\text{and}\quad (X \times Y)_{s,t} = (X_{s,y} \times Y_{s,t}).
\]
Analogously, the \defn{tensor product} \(V \ot W\) of two persistence modules is defined by
\[
(M \ot N)_r = M_r \ot N_r \quad\text{and}\quad (M \ot N)_{s,t} = (M_{s,y} \ot N_{s,t}).
\]

%For a general cohomology operation there is no formula expressing its action on the product of two cellular \(\R\)spaces in terms of its action on its factors, but for Steenrod operations there is.

From the naturality of the K\"unneth isomorphism and the Cartan relations we have the following.

\medskip\lemma
Let $X$ and $Y$ be pointed cellular $\R$-spaces.
The total Steenrod operations satisfy:
%For cohomology with coefficients in \(\Ftwo\) and \(\Fp\) respectively one has:
\begin{align*}
	\img_\Sq(X \times Y) &\cong \img_\Sq(X) \ot \img_\Sq(Y),
	&\img_\rP(X \times Y) &\cong \img_\rP(X) \ot \img_\rP(Y),\\
	\ker_\Sq(X \times Y) &\cong \ker_\Sq(X) \ot \ker_\Sq(Y),
	&\ker_\rP(X \times Y) &\cong \ker_\rP(X) \ot \ker_\rP(Y).
\end{align*}

\subsubsection{}

Given two metric spaces $\cX$ and $\cY$.
The \defn{$\ell^\infty$ metric} on $\cX \times \cY$ is defined by
\[
d(x \times y, \, x' \times y') = \max\set{d(x,x'), d(y,y')}.
\]

\medskip\theorem
Let $\cX$ and $\cY$ be metric spaces.
The total Steenrod operations satisfy:
\begin{align*}
	&\img^{\VR}_\Sq(\cX \times \cY) \cong \img^{\VR}_\Sq(\cX) \ot \img^{\VR}_\Sq(\cY), \\
	&\ker^{\VR}_\Sq(\cX \times \cY) \cong \ker^{\VR}_\Sq(\cX) \ot \ker^{\VR}_\Sq(\cY), \\
	&\img^{\VR}_\rP(\cX \times \cY) \cong \img^{\VR}_\rP(\cX) \ot \img^{\VR}_\rP(\cY), \\
	&\ker^{\VR}_\rP(\cX \times \cY) \cong \ker^{\VR}_\rP(\cX) \ot \ker^{\VR}_\rP(\cY),
\end{align*}
where \(\cX \times \cY\) is equipped with the \(\ell^\infty\) metric.

%\medskip\corollary
%For any two metric spaces $\cX$ and $\cY$.
%\begin{align*}
%	\img\Sq^k_{\VR\cX \times \VR\cY} &\cong\, \img\sum_{\mathclap{i+j=k}} \Sq^i_{\VR\cX} \ot \Sq^j_{\VR\cY}\,, \\ \ker\Sq^k_{\VR\cX \times \VR\cY} &\cong\, \ker\sum_{\mathclap{i+j=k}} \Sq^i_{\VR\cX} \ot \Sq^j_{\VR\cY}\,, \\
%	\img\rP^k_{\VR\cX \times \VR\cY} &\cong\, \img\sum_{\mathclap{i+j=k}} \rP^i_{\VR\cX} \otimes \rP^j_{\VR\cY}\,, \\
%	\ker\rP^k_{\VR\cX \times \VR\cY} &\cong\, \ker\sum_{\mathclap{i+j=k}} \rP^i_{\VR\cX} \otimes \rP^j_{\VR\cY}\,,
%\end{align*}
%for any $k \in \N$.

\begin{proof}
	This follows from the previous lemma and the proof of \cite[Thm.~6.1(1)]{lim2024vietoris}, which constructs a natural isomorphism $\rH^\VR(\cX) \ot \rH^\VR(\cY) \cong \rH^\VR(\cX \times \cY)$ when the metric is \(\ell^\infty\).
\end{proof}